lock acquire and release

pulse/ulib/experimental/Steel.Memory.fst
@@ -558,7 +558,7 @@ let rec affine_star_aux (p:hprop) (m:heap) (m':heap { disjoint m m' })
 
 let affine_star (p q:hprop) (m:heap)
   : Lemma
-    (ensures (interp (p `star` q) m ==> interp p m))
+    (ensures (interp (p `star` q) m ==> interp p m /\ interp q m))
   = ()
 
 ////////////////////////////////////////////////////////////////////////////////
@@ -869,3 +869,156 @@ let new_lock_action (p:hprop)
   : m_action p (lock p) (fun _ -> emp)
   = new_lock_is_frame_preserving p;
     new_lock_pre_m_action p
+
+////////////////////////////////////////////////////////////////////////////////
+assume
+val get_lock (l:lock_store) (i:nat{i < L.length l})
+  : (prefix : lock_store &
+     li : lock_state &
+     suffix : lock_store {
+       l == L.(prefix @ (li::suffix)) /\
+       L.length (li::suffix) == i + 1
+     })
+
+let lock_i (l:lock_store) (i:nat{i < L.length l}) : lock_state =
+  let (| _, li, _ |) = get_lock l i in
+  li
+
+assume
+val lock_store_invariant_append (l1 l2:lock_store)
+  : Lemma (lock_store_invariant (l1 @ l2) `equiv`
+           (lock_store_invariant l1 `star` lock_store_invariant l2))
+
+let hprop_of_lock_state (l:lock_state) : hprop =
+  match l with
+  | Available p -> p
+  | Locked p -> p
+
+let lock_ok (#p:hprop) (l:lock p) (m:mem) =
+  l < L.length m.locks /\
+  hprop_of_lock_state (lock_i m.locks l) == p
+
+let lock_store_evolves : Preorder.preorder lock_store =
+  fun (l1 l2 : lock_store) ->
+    L.length l2 >= L.length l1 /\
+    (forall (i:nat{i < L.length l1}).
+       hprop_of_lock_state (lock_i l1 i) ==
+       hprop_of_lock_state (lock_i l2 i))
+
+let mem_evolves : Preorder.preorder mem =
+  fun m0 m1 -> lock_store_evolves m0.locks m1.locks
+
+let lock_ok_stable (#p:_) (l:lock p) (m0 m1:mem)
+  : Lemma (lock_ok l m0 /\
+           m0 `mem_evolves` m1 ==>
+           lock_ok l m1)
+  = ()
+
+let pure (p:prop) : hprop = refine emp (fun _ -> p)
+
+let intro_pure (p:prop) (q:hprop) (h:hheap q { p })
+  : hheap (pure p `star` q)
+  = emp_unit q;
+    star_commutative q emp;
+    h
+
+let intro_hmem_or (p:prop) (q:hprop) (h:hmem q)
+  : hmem (h_or (pure p) q)
+  = h
+
+let middle_to_head (p q r:hprop) (h:hheap (p `star` (q `star` r)))
+  : hheap (q `star` (p `star` r))
+  = star_associative p q r;
+    star_commutative p q;
+    star_associative q p r;
+    h
+
+let maybe_acquire #p (l:lock p) (m:mem { lock_ok l m } )
+  : (b:bool &
+     m:hmem (h_or (pure (b == false)) p))
+  = let (| prefix, li, suffix |) = get_lock m.locks l in
+    match li with
+    | Available _ ->
+      let h = heap_of_mem m in
+      assert (interp (lock_store_invariant m.locks) h);
+      lock_store_invariant_append prefix (li::suffix);
+      assert (lock_store_invariant m.locks `equiv`
+             (lock_store_invariant prefix `star`
+                      (p `star` lock_store_invariant suffix)));
+      assert (interp (lock_store_invariant prefix `star`
+                       (p `star` lock_store_invariant suffix)) h);
+      let h = middle_to_head (lock_store_invariant prefix) p (lock_store_invariant suffix) h in
+      assert (interp (p `star`
+                        (lock_store_invariant prefix `star`
+                         lock_store_invariant suffix)) h);
+      let new_lock_store = prefix @ (Locked p :: suffix) in
+      lock_store_invariant_append prefix (Locked p :: suffix);
+      assert (lock_store_invariant new_lock_store `equiv`
+              (lock_store_invariant prefix `star`
+                         lock_store_invariant suffix));
+      equiv_star_left p (lock_store_invariant new_lock_store)
+                        (lock_store_invariant prefix `star`
+                          lock_store_invariant suffix);
+      assert (interp (p `star` lock_store_invariant new_lock_store) h);
+      let h : hheap (p `star` lock_store_invariant new_lock_store) = h in
+      assert (heap_of_mem m == h);
+      star_commutative p (lock_store_invariant new_lock_store);
+      affine_star (lock_store_invariant new_lock_store) p h;
+      assert (interp (lock_store_invariant new_lock_store) h);
+      let mem : hmem p = { m with locks = new_lock_store } in
+      let b = true in
+      let mem : hmem (h_or (pure (b==false)) p) = intro_hmem_or (b == false) p mem in
+      (| b, mem |)
+
+    | Locked _ ->
+      let b = false in
+      assert (interp (pure (b == false)) (heap_of_mem m));
+      let h : hheap (mem_invariant m) = heap_of_mem m in
+      let h : hheap (pure (b==false) `star` mem_invariant m) =
+        intro_pure (b==false) (mem_invariant m) h in
+      intro_or_l (pure (b==false) `star` mem_invariant m)
+                 (p `star` mem_invariant m)
+                 h;
+      or_star (pure (b==false)) p (mem_invariant m) h;
+      assert (interp (h_or (pure (b==false)) p `star` mem_invariant m) h);
+      (| false, m |)
+
+#push-options "--query_stats --z3rlimit_factor 8"
+let release #p (l:lock p) (m:hmem p { lock_ok l m } )
+  : (b:bool &
+     hmem emp)
+  = let (| prefix, li, suffix |) = get_lock m.locks l in
+    let h = heap_of_mem m in
+    lock_store_invariant_append prefix (li::suffix);
+    assert (interp (p `star`
+                     (lock_store_invariant prefix `star`
+                       (lock_store_invariant (li::suffix)))) h);
+    match li with
+    | Available _ ->
+      (* this case is odd, but not inadmissible.
+         We're releasing a lock that was not previously acquired.
+         We could either fail, or just silently proceed.
+         I choose to at least signal this case in the result
+         so that we can decide to fail if we like, at a higher layer *)
+      emp_unit_left (lock_store_invariant m.locks);
+      let mem : hmem emp = m in
+      (| false, mem |)
+
+    | Locked _ ->
+      assert (interp (p `star`
+                        (lock_store_invariant prefix `star`
+                          (lock_store_invariant suffix))) h);
+      let h = middle_to_head p (lock_store_invariant prefix) (lock_store_invariant suffix) h in
+      assert (interp (lock_store_invariant prefix `star`
+                        (p `star`
+                          (lock_store_invariant suffix))) h);
+      let new_lock_store = prefix @ (Available p :: suffix) in
+      lock_store_invariant_append prefix (Available p :: suffix);
+      assert (lock_store_invariant new_lock_store `equiv`
+                (lock_store_invariant prefix `star`
+                 (p `star` lock_store_invariant (suffix))));
+      assert (interp (lock_store_invariant new_lock_store) h);
+      emp_unit_left (lock_store_invariant new_lock_store);
+      let mem : hmem emp = { m with locks = new_lock_store } in
+      (| true, mem |)
+#pop-options
